mostly the proof

memabs/CohRefine.v
@@ -10,25 +10,41 @@ Require Import SemDef.
 Section LTS.
   Context {liA liB S} (L : lts liA liB S).
 
-  Inductive lts_ext_calls : S -> token (!liA) -> S -> Prop :=
-  | lts_ext_nil: forall s,
-      lts_ext_calls s nil s
+  (* a sequence of external calls with no internal steps in between
+     but we allow internal steps at the beginning and end *)
+  Inductive lts_ext_calls : bool -> S -> token (!liA) -> bool -> S -> Prop :=
+  | lts_ext_nil: forall s s',
+      Star L s E0 s' ->
+      lts_ext_calls false s nil false s'
   | lts_ext_cons: forall s s' s'' q r t,
       Smallstep.at_external L s q ->
       Smallstep.after_external L s r s' ->
-      lts_ext_calls s' t s'' ->
-      lts_ext_calls s ((q, r) :: t) s''.
+      lts_ext_calls false s' t false s'' ->
+      lts_ext_calls false s ((q, r) :: t) false s''
+  | lts_ext_init: forall s s' s'' t,
+      Star L s E0 s' ->
+      lts_ext_calls false s' t false s'' ->
+      lts_ext_calls true s t false s''.
 
   Lemma lts_trace_concat s s' t1 t2 r:
-    lts_ext_calls s t1 s' ->
+    lts_ext_calls true s t1 false s' ->
     lts_trace L false s' t2 r ->
-    lts_trace L false s (t1 ++ t2) r.
+    lts_trace L true s (t1 ++ t2) r.
   Proof.
-    intros H. induction H.
-    - auto.
-    - intros H'. specialize (IHlts_ext_calls H').
-      rewrite <- app_comm_cons. econstructor; eauto.
-      eapply lts_trace_steps. eapply Smallstep.star_refl. auto.
+    intros H.
+    eapply lts_ext_calls_ind
+      with (P := fun b s t b' s' => lts_trace L false s' t2 r -> lts_trace L true s (t ++ t2) r).
+    - intros. eapply lts_trace_steps; eauto.
+    - intros until t. intros Hext Haft Hcalls IH H'.
+      specialize (IH H'). rewrite <- app_comm_cons.
+      eapply lts_trace_steps. eapply Smallstep.star_refl.
+      eapply lts_trace_external; eauto.
+    - intros until t. intros Hstar Hcalls IH H'.
+      specialize (IH H').
+      inv IH.
+      eapply lts_trace_steps; [ | eauto ].
+      eapply Smallstep.star_trans; eauto.
+    - eauto.
   Qed.
 End LTS.
 
@@ -40,6 +56,7 @@ Lemma trace_split {liA liB: language_interface} (σ: !liA --o !liB) q t r rest:
   exists t1 t2, t = t1 ++ t2 /\
            exec σ q t1 r /\
            has (next σ t1 q r) (t2, rest).
+Admitted.
 (* Proof. *)
 (*   intros H. *)
 (*   assert (H': exists t', has σ (t', (q,r) :: nil)). *)
@@ -66,8 +83,49 @@ Section REFINE.
     inversion Htop as [? s0 ? ? Hvq Hinit Htrace]. subst.
     econstructor; [ apply Hvq | econstructor; apply Hinit | ].
     clear Hvq Hinit Htop. clear T1 H T2.
-    revert mid_tr_d bottom_tr Σ Hmid Hbot.
-    induction Htrace.
-    admit. admit.
+    remember (Σ se) as σ. clear Heqσ.
+    revert mid_tr_d bottom_tr σ Hmid Hbot.
+    eapply lts_trace_ind
+      with (P := fun b s t r =>
+             forall (mid_tr_d : list (d_query * d_reply)) (bottom_tr : token (!li_d))
+               (σ : !li_d --o !li_d),
+               dag_lmaps li_dc mid_tr_d t ->
+               has σ (bottom_tr, mid_tr_d) ->
+               lts_trace (Abs.lts Σ (semantics1 C) li_rel se) true (Abs.st (semantics1 C) s σ) bottom_tr r).
+    4: {  apply Htrace. }
+    - intros until r. intros Hstar H IH.
+      intros ? ? ? Hmid Hbot. specialize (IH _ _ _ Hmid Hbot).
+      inversion IH as [? s1 ? ? Hstar' | | ]. subst.
+      eapply lts_trace_steps; [ | eauto].
+      eapply Smallstep.star_trans; eauto.
+      2: { instantiate (1 := E0). auto. }
+      clear -Hstar. induction Hstar.
+      + eapply Smallstep.star_refl.
+      + eapply Smallstep.star_left; eauto.
+        eapply Abs.step_internal; eauto.
+    - intros. eapply lts_trace_steps.
+      eapply Smallstep.star_refl.
+      inv H0. assert (bottom_tr = nil). admit.
+      subst. eapply lts_trace_final.
+      eapply Abs.final_state_intro. auto.
+    - intros s qx rx s' t r Hext Haft H' IH.
+      intros ? ? ? Hmid Hbot.
+      inversion Hmid as [| [qd rd] [? ?] mid_tr_d' mid_tr_c' Hq Hmid']. subst.
+      eapply trace_split in Hbot as (t1 & t2 & Ht & Hexec & Hnext).
+      subst bottom_tr.
+      specialize (IH _ _ _ Hmid' Hnext).
+      inversion IH as [? s1 ? ? Hstar | | ]. subst.
+      eapply lts_trace_concat; eauto.
+      eapply lts_ext_init.
+      eapply Smallstep.star_one. eapply Abs.step_at_external; eauto.
+      clear -Hstar.
+      remember (next σ t1 qd rd) as σ'. clear Heqσ'.
+      induction t1.
+      + eapply lts_ext_nil.
+        eapply Smallstep.star_left. eapply Abs.step_after_external.
+        eapply Hstar. auto.
+      + destruct a as [qx rx].
+        eapply lts_ext_cons.
+        constructor. econstructor. apply IHt1.
 
-  End REFINE.
+End REFINE.
